examples/Incubator_locales.thy
@@ -1,0 +1,64 @@
+section \<open> Incubator \<close>
+
+theory Incubator_locales
+  imports "Z_Machines.Z_Machine"
+begin
+
+consts MAX_TEMP :: \<int>
+consts MIN_TEMP :: \<int>
+
+definition "TEMP = {MIN_TEMP..MAX_TEMP}"
+
+def_consts 
+  MAX_TEMP = 30
+  MIN_TEMP = 15
+
+zstore IncubatorMonitor = 
+  temp :: \<int>
+  where mintemp: "MIN_TEMP \<le> temp" maxtemp: "temp \<le> MAX_TEMP"
+
+zoperation Increment =
+  over IncubatorMonitor
+  pre "temp < MAX_TEMP"
+  update "[temp\<Zprime> = temp + 1]"
+
+lemma Increment_correct: "\<^bold>{IncubatorMonitor_inv\<^bold>} Increment() \<^bold>{IncubatorMonitor_inv\<^bold>}"
+  unfolding Increment_def IncubatorMonitor_inv_def  
+proof (hoare_wlp_auto)
+  fix temp
+  assume pres: "temp < MAX_TEMP" and inv: "IncubatorMonitor temp" 
+  then interpret IncubatorMonitor temp
+    by simp
+  show "IncubatorMonitor (temp + 1)"
+  proof
+    show "MIN_TEMP \<le> temp + 1"
+      using mintemp by auto
+    show "temp + 1 \<le> MAX_TEMP"
+      by (simp add: add1_zle_eq pres)
+  qed
+qed
+
+zoperation Decrement =
+  over IncubatorMonitor
+  pre "temp > MIN_TEMP" \<comment> \<open> Change to @{term "(temp \<ge> MIN_TEMP)\<^sub>e"} to break the invariant \<close>
+  update "[temp\<Zprime> = temp - 1]"
+
+lemma Decrement_correct: "\<^bold>{IncubatorMonitor_inv\<^bold>} Decrement() \<^bold>{IncubatorMonitor_inv\<^bold>}"
+  unfolding Decrement_def IncubatorMonitor_inv_def IncubatorMonitor_def by hoare_wlp
+
+zoperation GetTemp =
+  over IncubatorMonitor
+  params currentTemp \<in> TEMP
+  where "temp = currentTemp"
+
+lemma GetTemp_correct: "\<^bold>{IncubatorMonitor_inv\<^bold>} GetTemp v \<^bold>{IncubatorMonitor_inv\<^bold>}"
+  unfolding GetTemp_def IncubatorMonitor_inv_def IncubatorMonitor_def by hoare_wlp
+
+zmachine Incubator =
+  init "[temp \<leadsto> 20]"
+  operations Increment Decrement GetTemp
+
+animate Incubator
+
+end
+  
